theories/LKID.v
@@ -89,18 +89,32 @@ Section lkid.
       LKID (shift_formulas Γ ⊢ φ :: shift_formulas Δ) ->
       LKID (Γ ⊢ (FAll φ) :: Δ)
   | IndL : forall Γ Δ (Pj : IndPredS Σ) (u : vec (term Σ) (indpred_ar Pj))
-             (z_i : forall P, vec var (indpred_ar P))
+             (z_i : forall P, vec var (indpred_ar P)) (* dodati pretpostavku forall P, NoDup (z_i P)? *)
              (G_i : IndPredS Σ -> formula Σ)
              (HG2 : forall Pi, ~mutually_dependent Pi Pj -> G_i Pi = FIndPred Pi (V.map var_term (z_i Pi))),
+      let maxΓ := max_fold (map some_var_not_in_formula Γ) in
+      let maxΔ := max_fold (map some_var_not_in_formula Δ) in
+      let maxP := some_var_not_in_formula (FIndPred Pj u) in
+      let shift_factor := max maxP (max maxΓ maxΔ) in
+      let Fj := subst_formula (finite_subst (z_i Pj) u) (G_i Pj) in
       let minor_premises :=
         (forall pr (Hdep : mutually_dependent (indcons pr) Pj),
-            LKID (
-                (* Qovi *) FPreds_from_preds (preds pr) ++
-                  (* Govi *) map (fun p => subst_formula (finite_subst (z_i (p .1)) (p .2)) (G_i (p .1))) (indpreds pr) ++ Γ
-                  ⊢ subst_formula (finite_subst (z_i (indcons pr)) (indargs pr)) (G_i (indcons pr)) :: Δ))
-      in          (* TODO treba shiftati Γ i Δ za najvecu varijablu koja se javlja u ?negdje? *)
+            let Qs := shift_formulas_by shift_factor (FPreds_from_preds (preds pr)) in
+            let Gs := map (fun p =>
+                             let P := p.1 in
+                             let args := p.2 in
+                             let shifted_args := V.map (shift_term_by shift_factor) args in
+                             let σ := finite_subst (z_i P) (shifted_args) in
+                             let G := G_i P in
+                             subst_formula σ G)
+                        (indpreds pr) in
+            let Pi := indcons pr in
+            let tx := V.map (shift_term_by shift_factor) (indargs pr) in
+            let Fi := subst_formula (finite_subst (z_i Pi) tx) (G_i Pi) in
+            LKID (Qs ++ Gs ++ Γ ⊢ Fi :: Δ))
+      in
       minor_premises ->
-      LKID (subst_formula (finite_subst (z_i Pj) u) (G_i Pj) :: Γ ⊢ Δ) ->
+      LKID (Fj :: Γ ⊢ Δ) ->
       LKID (FIndPred Pj u :: Γ ⊢ Δ)
   | IndR : forall Γ Δ pr σ,
       Φ pr ->
